\documentclass[]{article}

\usepackage{amsmath}
\usepackage[margin=.75in]{geometry}

\begin{document}

\title{CS 161 - Assignment 5}
\author{Lowell Bander}
\maketitle

\section{}
\begin{table}[h]
\centering
\begin{tabular}{ c | c | c | c }
$P$ & $Q$ & $P \implies \neg Q$  & $Q \implies \neg P$ \\\hline
F & F & T & T\\
F & T & T & T\\
T & F & T & T\\
T & T & F & F\\
\end{tabular}
\caption{Equivalence of $P \implies \neg Q$  and $Q \implies \neg P$.}
\end{table}

\begin{table}[h]
\centering
\begin{tabular}{ c | c | c | c }
$P$ & $Q$ & $P \iff \neg Q$  & $((P \land \neg Q) \lor (\neg P \land Q))$ \\\hline
F & F & F & F\\
F & T & T & T\\
T & F & T & T\\
T & T & F & F\\
\end{tabular}
\caption{Equivalence of $P \iff \neg Q$  and $((P \land \neg Q) \lor (\neg P \land Q))$.}
\end{table}

\newpage

\section{}

\begin{table}[h]
\centering
\begin{tabular}{ c | c | c | c | c}
$S$ & $F$ & $S \implies F$ & $\neg S \implies \neg F$ & $((S \implies F) \implies (\neg S \implies \neg F))$ \\\hline
F & F & T & T & T\\
F & T & T & F & F\\
T & F & F & T & T\\
T & T & T & T & T\\
\end{tabular}
\caption{The sentence $((S \implies F) \implies (\neg S \implies \neg F))$ is observed to be satisfiable yet invalid.}
\end{table}

\begin{table}[h!]
\centering
\begin{tabular}{ c | c | c | c | c | c}
$S$ & $F$ & $H$ & $S \implies F$ & $(S \lor H) \implies F$ & $((S \implies F) \implies ((S \lor H) \implies F))$ \\\hline
F & F & F & T & T & T \\
F & F & T & T & F & F \\
F & T & F & T & T & T \\
F & T & T & T & T & T \\
T& F & F & F & F & T \\
T & F & T & F & F & T \\
T & T & F & T & T & T \\
T & T & T & T & T & T \\
\end{tabular}
\caption{The sentence $((S \implies F) \implies ((S \lor H) \implies F))$ is observed to be satisfiable yet invalid.}
\end{table}

\begin{table}[h!]
\centering
\begin{tabular}{ c | c | c | c | c | c}
$S$ & $F$ & $H$ & $((S \land H) \implies F)$  & $((S \implies F) \lor (H \implies F))$ & $((S \land H) \implies F) \iff ((S \implies F) \lor (H \implies F))$\\\hline
F & F & F & T & T & T \\
F & F & T & T & T & T \\
F & T & F & T & T & T \\
F & T & T & T & T & T \\
T& F & F & T & T & T\\
T & F & T & F & F & T \\
T & T & F & T & T & T \\
T & T & T & T & T & T \\
\end{tabular}
\caption{The sentence $((S \land H) \implies F) \iff ((S \implies F) \lor (H \implies F))$ is observed to be both satisfiable and valid.}
\end{table}

\newpage

\section{}

If we assign the state of being mythical to $Y$, mortal to $O$, mammal to $A$, horned to $H$, and magical to $G$, the information can be represented with the following propositional logic knowledge base:

\begin{itemize}
\item{$Y \implies \neg Q$}
\item{$\neg Y \implies (O \land A)$}
\item{$(\neg O \lor A) \implies H$}
\item{$H \implies G$}
\end{itemize}

The representation of this knowledge base in conjunctive normal form is

\begin{gather}
(\neg Y \lor \neg O) \land (Y \lor O) \land (Y \lor A) \land (O \lor \neg A \lor H) \land (\neg H \lor G)
\end{gather}

\end{document}
